Add syntax for natural numbers

syntax.sig
@@ -13,3 +13,7 @@ tBool : tm
 tEq : tm -> tm -> tm -> tm
 tJ : tm -> tm -> tm -> tm -> tm
 tRefl : tm
+tNat : tm
+tInd : (tm -> tm) -> tm -> (tm -> tm -> tm) -> tm -> tm
+tZero : tm
+tSuc : tm -> tm
